Bit of tydiying

theories/Interp/Sched.v
@@ -9,9 +9,6 @@ Import ITree.Basics.Basics.Monads.
 Import MonadNotation.
 Open Scope monad_scope.
 
-#[global] Instance ctree_trigger {E} : MonadTrigger E (ctree E) :=
-  @CTree.trigger _.
-
 #[global] Instance stateT_trigger {E S M} {MM : Monad M} {MT: MonadTrigger E M} :
   MonadTrigger E (stateT S M) :=
   fun _ e s => v <- mtrigger _ e;; ret (s, v).
@@ -27,6 +24,25 @@ Definition schedule {E M : Type -> Type}
 				    | @ChoiceF _ _ _ _ n k => bind (h n) (fun x => ret (inl (k x)))
 				    | VisF e k => bind (mtrigger _ e) (fun x => ret (inl (k x)))
 				    end).
+
+Variant pureb {E X} (rec : ctree E X -> Prop) : ctree' E X -> Prop :=
+  | pure_ret   (v : X) : pureb rec (RetF v)
+  | pure_delay n k (REC: forall v, rec (k v)) : pureb rec (ChoiceIF n k).
+#[global] Hint Constructors equb: core.
+
+Definition pureb_ {E X} rec (t : ctree E X) := pureb rec (observe t).
+
+Program Definition fpure {E R} : mon (ctree E R -> Prop) := {|body := pureb_|}.
+Next Obligation.
+  red in H0 |- *.
+  inversion_clear H0; econstructor; auto.
+Qed.
+
+Definition pure {E R} := gfp (@fpure E R).
+
+(* Definition schedule_pure {E} (hV hI : forall n, fin n) : ctree E ~> ctree E := *)
+(*   schedule (fun n => Ret (h n)). *)
+
 
 Definition schedule_cst {E} (h : forall n, fin n) : ctree E ~> ctree E :=
   schedule (fun n => Ret (h n)).
@@ -46,321 +62,3 @@ Definition round_robin {E} : ctree E ~> stateT nat (ctree E).
   apply (NPeano.Nat.mod_upper_bound).
   auto with arith.
 Defined.
-
-(* TODO:
-Can we do something with a stream?
-One round robin per arity?
-Random scheduler on the OCaml side?
-Fairness? Too low level here I think? Maybe at the level of Imp.
-Prove that the original computation simulates the scheduled one?
-*)
-
-
-(* TODO: move, use globally? *)
-Notation ChoiceVF := (ChoiceF true).
-Notation ChoiceIF := (ChoiceF false).
-
-Definition guarded_form {E X} (t : ctree E X) : ctree E X :=
-	CTree.iter (fun t =>
-				        match observe t with
-				        | RetF r => ret (inr r)
-				        | ChoiceIF n k =>
-                    ChoiceI n (fun x => Ret (inl (k x)))
-				        | ChoiceVF n k =>
-                    ChoiceI n (fun x => TauV (Ret (inl (k x))))
-				        | VisF e k => bind (mtrigger _ e) (fun x => Ret (inl (k x)))
-				        end) t.
-
-Lemma unfold_guarded_form {E X} (t : ctree E X) :
-  guarded_form t ≅
-  match observe t with
-	| RetF r => ret r
-	| ChoiceIF n k =>
-      ChoiceI n (fun x => TauI (guarded_form (k x)))
-	| ChoiceVF n k =>
-      ChoiceI n (fun x => TauV (TauI (guarded_form (k x))))
-	| VisF e k => bind (mtrigger _ e) (fun x => TauI (guarded_form (k x)))
-	end.
-Proof.
-  unfold guarded_form at 1.
-  rewrite unfold_iter.
-  desobs t; cbn.
-  - now rewrite bind_ret_l.
-  - unfold mtrigger; rewrite bind_bind, !bind_trigger.
-    step; constructor; intros ?.
-    rewrite bind_ret_l.
-    reflexivity.
-  - destruct vis.
-    + rewrite bind_choice.
-      step; constructor; intros ?.
-      rewrite bind_tauV; step; constructor; intros ?.
-      rewrite bind_ret_l.
-      step; constructor; auto.
-    + rewrite bind_choice.
-      step; constructor; intros ?.
-      rewrite bind_ret_l.
-      step; constructor; auto.
-Qed.
-
-Lemma foo {E X} l (t t' u : ctree E X):
-  t ~ t' ->
-  trans l t u ->
-  exists u', trans l t' u' /\ u ~ u'.
-Proof.
-  intros * EQ TR.
-  step in EQ; destruct EQ as [F _]; apply F in TR; destruct TR; eauto.
-Qed.
-
-Lemma trans_guarded_inv_strong :
-  forall {E X} (t u v : ctree E X) l,
-    (v ≅ guarded_form t \/ v ≅ TauI (guarded_form t)) ->
-    trans l v u ->
-    exists t', trans l t t'
-          /\ (u ≅ guarded_form t' \/ u ≅ TauI (guarded_form t')).
-Proof.
-  intros * EQ TR.
-  revert t EQ.
-  unfold trans in TR; repeat red in TR.
-  dependent induction TR.
-  - intros ? [EQ | EQ].
-    + rewrite ctree_eta, <- x, unfold_guarded_form in EQ.
-      setoid_rewrite (ctree_eta t).
-      desobs t; try now step in EQ; inv EQ.
-      destruct vis.
-      * pose proof equ_choice_invT _ _ EQ as [<- _].
-        apply equ_choice_invE with (x := x0) in EQ .
-        rewrite EQ in TR.
-        apply trans_tauV_inv in TR as [EQ' ->].
-        eexists; split; eauto.
-        etrans.
-
-      * pose proof equ_choice_invT _ _ EQ as [<- _].
-        apply equ_choice_invE with (x := x0) in EQ .
-        specialize (IHTR _ _ eq_refl eq_refl).
-        edestruct IHTR as (t' & ? & ?); eauto.
-        exists t'.
-        split.
-        eapply trans_choiceI with (x := x0); eauto.
-        eauto.
-
-    + rewrite ctree_eta, <- x in EQ.
-      pose proof equ_choice_invT _ _ EQ as [-> _].
-      apply equ_choice_invE with (x := x0) in EQ .
-      specialize (IHTR _ _ eq_refl eq_refl).
-      edestruct IHTR as (t' & ? & ?); eauto.
-
-  - (* G(t) ≅ ChoiceV k : absurd *)
-    intros ? [EQ | EQ].
-    + rewrite ctree_eta, <- x1, unfold_guarded_form in EQ.
-      desobs t0; try now step in EQ; inv EQ.
-      destruct vis; try now step in EQ; inv EQ.
-    + rewrite ctree_eta, <- x1 in EQ.
-      now step in EQ; inv EQ.
-
-  - (* G(t) ≅ Vis e k : t ≅ Vis e k', k x ≅ TauI (G (k' x)) *)
-    intros ? [EQ | EQ].
-    + setoid_rewrite (ctree_eta t0).
-      rewrite ctree_eta, <- x1, unfold_guarded_form in EQ.
-      rewrite (ctree_eta t), x in H.
-      clear t x.
-      desobs t0; try now step in EQ; inv EQ.
-      2:destruct vis; try now step in EQ; inv EQ.
-      cbn in *.
-      unfold mtrigger in EQ; rewrite bind_trigger in EQ.
-      pose proof equ_vis_invT _ _ _ _ EQ; subst.
-      pose proof equ_vis_invE _ _ _ _ EQ as [-> EQ'].
-      eexists; split.
-      etrans.
-      rewrite <- ctree_eta in H.
-      rewrite <- H.
-      rewrite EQ'.
-      auto.
-    + rewrite ctree_eta, <- x1 in EQ.
-      now step in EQ; inv EQ.
-
-  - (* G(t) ≅ Ret x : t ≅ Ret x *)
-    intros ? [EQ | EQ].
-    + setoid_rewrite (ctree_eta t).
-      rewrite ctree_eta, <- x0, unfold_guarded_form in EQ.
-      desobs t; try now step in EQ; inv EQ.
-      2:destruct vis; try now step in EQ; inv EQ.
-      step in EQ; inv EQ.
-      eexists; split.
-      etrans.
-      left.
-      rewrite ctree_eta, <- x, unfold_guarded_form.
-      cbn.
-      rewrite ! choiceI0_always_stuck.
-      reflexivity.
-    + rewrite ctree_eta, <- x0 in EQ.
-      now step in EQ; inv EQ.
-Qed.
-
-Lemma trans_guarded_inv :
-  forall E X (t u : ctree E X) l,
-    trans l (guarded_form t) u ->
-    exists t', trans l t t'
-          /\ u ~ guarded_form t'.
-Proof.
-  intros.
-  edestruct @trans_guarded_inv_strong as (t' & TR & EQ); [|eassumption|].
-  left; eauto.
-  exists t'; split; auto.
-  destruct EQ as [EQ |EQ]; rewrite EQ; auto.
-  rewrite sb_tauI; auto.
-Qed.
-
-Ltac fold_bind :=
-  repeat match goal with
-           |- context [CTree.subst ?k ?t] => fold (CTree.bind t k)
-         end.
-
-#[global] Instance guarded_equ E X : Proper (equ eq ==> equ eq) (@guarded_form E X).
-Proof.
-  do 2 red.
-  coinduction ? IH.
-  intros * EQ.
-  step in EQ.
-  rewrite ! unfold_guarded_form.
-  cbn*.
-  inv EQ; auto.
-  - cbn.
-    constructor; intros ?.
-    fold_bind; rewrite ! bind_ret_l.
-    step; constructor; intros _.
-    auto.
-  - destruct b; cbn.
-    all: constructor; intros ?.
-    all: repeat (step; constructor; intros ?).
-    all: auto.
-Qed.
-
-(* TODO: bind simpl never globally? *)
-(* TODO: Taus without continuation? *)
-(* TODO: tactic for better stepping for equ *)
-(* TODO: tactics for better stepping for sbisim (see a couple above) *)
-(* Equality on [observe u] rewritten in [equ]? *)
-Opaque CTree.bind.
-Lemma trans_guarded_strong :
-  forall E X (t u : ctree E X) l,
-    trans l t u ->
-    exists u',
-      trans l (guarded_form t) u'
-      /\ (u' ≅ guarded_form u
-         \/ u' ≅ TauI (guarded_form u)).
-Proof.
-  intros * TR.
-  (* revert t EQ. *)
-  unfold trans in TR; repeat red in TR.
-  dependent induction TR; intros.
-  - (* destruct EQ as [EQ | EQ]. *)
-    edestruct IHTR as (u' & TR' & EQ'); eauto.
-    setoid_rewrite unfold_guarded_form at 1; rewrite <- x.
-    exists u'; split.
-    eapply trans_choiceI with (x := x0); [| reflexivity].
-    now apply trans_tauI.
-    auto.
-  - setoid_rewrite unfold_guarded_form at 1; rewrite <- x1.
-    eexists; split.
-    eapply trans_choiceI with (x := x0); [| reflexivity].
-    etrans.
-    right.
-    step; constructor; intros ?.
-    rewrite H.
-    rewrite (ctree_eta t0),x,<- ctree_eta.
-    auto.
-  - setoid_rewrite unfold_guarded_form at 1; rewrite <- x1.
-    eexists; split.
-    unfold mtrigger, ctree_trigger; cbn.
-    rewrite bind_trigger.
-    etrans.
-    right.
-    step; constructor; intros ?.
-    rewrite H.
-    rewrite (ctree_eta t0),x,<- ctree_eta.
-    auto.
-  - setoid_rewrite unfold_guarded_form at 1; rewrite <- x0.
-    eexists; split.
-    (*
-      Why do I need to cbn even if I add:
-      Hint Unfold ret Monad_ctree : trans.
-     *)
-    cbn; etrans.
-    left.
-    rewrite unfold_guarded_form, <- x; cbn.
-    now rewrite ! choiceI0_always_stuck.
-Qed.
-
-Lemma trans_guarded :
-  forall E X (t u : ctree E X) l,
-    trans l t u ->
-    exists u',
-      trans l (guarded_form t) u'
-      /\ u' ~ guarded_form u.
-Proof.
-  intros * TR.
-  edestruct trans_guarded_strong as (u' & TR' & EQ'); eauto.
-  exists u'; split; auto.
-  destruct EQ' as [EQ' | EQ']; rewrite EQ'; auto.
-  now rewrite sb_tauI.
-Qed.
-
-(* TODO: define properly the set of tactics in [sbisim] and kill this.
-   TODO: this is not resilient enough, it loops if the goal is not exactly of the right shape
- *)
-Ltac sret  := apply step_sb_ret.
-Ltac svis  := apply step_sb_vis.
-Ltac stauv := apply step_sb_tauV.
-Ltac sstep := sret || svis || stauv.
-
-Lemma guarded_is_bisimilar {E X} : forall (t : ctree E X),
-    guarded_form t ~ t.
-Proof.
-  coinduction ? IH.
-  intros t.
-  rewrite (ctree_eta t) at 2.
-  rewrite unfold_guarded_form.
-  desobs t.
-  - now cbn.
-  - cbn*.
-    unfold mtrigger; rewrite bind_trigger.
-    sstep; intros ?.
-    rewrite sb_tauI.
-    apply IH.
-  - destruct vis.
-    + cbn.
-      split; intros ? ? TR.
-      * inv_trans.
-        subst.
-        eexists.
-        eapply trans_choiceV with (x := n0).
-        rewrite EQ.
-        rewrite sb_tauI.
-        apply IH.
-      * cbn.
-        inv_trans; subst.
-        eexists.
-        eapply trans_choiceI with (x := n0).
-        2:etrans.
-        etrans.
-        rewrite sb_tauI.
-        rewrite EQ; apply IH.
-    + split.
-      * intros ? ? TR.
-        cbn.
-        inv_trans.
-        edestruct trans_guarded_inv as (u' & TR' & EQ'); eauto.
-        eexists.
-        eapply trans_choiceI with (x := n0); [| reflexivity].
-        eassumption.
-        rewrite EQ'; auto.
-      * cbn; intros ? ? TR.
-        inv_trans.
-        edestruct trans_guarded as (u' & TR' & EQ'); eauto.
-        eexists.
-        eapply trans_choiceI with (x := n0); [| reflexivity].
-        apply trans_tauI.
-        eauto.
-        rewrite EQ'; auto.
-Qed.
-
